Add encoding of [zipper]. Fix tactic SIMP_specify.

test/coq/splay_proof.v
@@ -4,6 +4,10 @@ From osiris.proofmode Require Export proofmode. (* TODO *)
 From osiris.libs Require Import Stdlib.
 From test Require Import splay.
 
+(* -------------------------------------------------------------------------- *)
+
+(* Boilerplate: reflect the algebraic data type ['a tree]. *)
+
 Inductive tree (A : Type) : Type :=
 | Leaf: tree A
 | Node: tree A → A → tree A → tree A.
@@ -28,13 +32,56 @@ Fixpoint encode_tree `{Encode A} (t : tree A) : val :=
 Local Instance Encode_tree `{Encode A} : Encode (tree A) :=
   { encode := encode_tree }.
 
+(* -------------------------------------------------------------------------- *)
+
+(* Boilerplate: reflect the algebraic data type ['a zipper]. *)
+
+Inductive zipper (A : Type) : Type :=
+| Root  : zipper A
+| NodeL : zipper A → A → tree A → zipper A
+| NodeR : tree A → A → zipper A → zipper A.
+
+Arguments Root  {A}.
+Arguments NodeL {A} z1 x t2.
+Arguments NodeR {A} t1 x z2.
+
+Fixpoint encode_zipper `{Encode A} (z : zipper A) : val :=
+  match z with
+  | Root =>
+      VConstant "Root"
+  | NodeL z1 x t2 =>
+      let vs :=
+        VCons (encode_zipper z1) $
+        VCons (encode x) $
+        VCons (encode_tree t2) $
+        VNil
+      in
+      VData "NodeL" (VTuple vs)
+  | NodeR t1 x z2 =>
+      let vs :=
+        VCons (encode_tree t1) $
+        VCons (encode x) $
+        VCons (encode_zipper z2) $
+        VNil
+      in
+      VData "NodeR" (VTuple vs)
+  end.
+
+Local Instance Encode_zipper `{Encode A} : Encode (zipper A) :=
+  { encode := encode_zipper }.
+
+(* -------------------------------------------------------------------------- *)
+
+(* WIP *)
+
 Ltac SIMP_specify x φ :=
-  lazymatch goal with |- SIMP (dconcatenating ?δ _) =>
-    let o := eval cbn in (lookup_name δ x) in
-    lazymatch o with ret ?v =>
-      let h := fresh in
-      assert (φ v) as h; [| revert h; generalize v ]
-    end
+  lazymatch goal with
+  | |- SIMP (bind (dconcatenating ?δ _) _) _ =>
+      let o := eval cbn in (lookup_name δ x) in
+      lazymatch o with ret ?v =>
+        let h := fresh in
+        assert (φ v) as h; [| revert h; generalize v ]
+      end
   end.
 
 Lemma SIMP_simp_bind X Y (_ : Encode Y)
@@ -55,8 +102,5 @@ Lemma Splay__spec:
 Proof.
   intros.
   SIMP.
-  (* eapply SIMP_simp_bind. *)
-  (* Unset Printing Notations. *)
-  (* SIMP_bind. *)
-  (* SIMP_specify "splay" (λ (splay : val), True). *)
+  SIMP_specify "splay" (λ (splay : val), True).
 Abort.
